{
 "cells": [
  {
   "cell_type": "markdown",
   "id": "1cd1539b",
   "metadata": {},
   "source": [
    "## Problem 7.11\n",
    "\n",
    "The global weak form of the dynamic heat equation is given in Eqn. 7.80 as \n",
    "\n",
    "\\begin{equation*}\n",
    "    \\int_0^1 \\tilde{\\theta} \\, \\partial_t \\theta \\: \\mathrm{d}x = - \\int_0^1 \\alpha\\, ( \\partial_x\\tilde{\\theta} )\\,( \\partial_x\\theta ) \\: \\mathrm{d}x \\: + \\: \\int_0^1 \\tilde{\\theta}\\, h\\, \\mathrm{d}x \\: + \\alpha\\, \\tilde{\\theta} \\, \\partial_x \\theta \\, |_0^1 \\quad. \n",
    "\\end{equation*}\n",
    "\n",
    "\n",
    "Writing the temperature field, $\\theta(x,\\,t)$, and test function, $\\tilde{\\theta}(x,\\,t)$, as in Eqns 7.26 and 7.23, \n",
    "\n",
    "\\begin{align*}\n",
    "\\theta(x,\\,t) &= \\sum_{B=1}^n d_B\\,N_B(x) \\:+\\: \\theta_1 N_{n+1}(x)\\\\\n",
    "\\tilde{\\theta}(x,\\,t) &= \\sum_{A=1}^n c_A\\,N_A(x)\n",
    "\\end{align*}\n",
    "\n",
    "we may then express the temporal gradients of these functions: \n",
    "\n",
    "\n",
    "\\begin{align*}\n",
    "\\partial_t \\theta(x,\\,t) &= \\sum_{B=1}^n \\dot{d}_B\\,N_B(x) \\quad, \\\\\n",
    "\\partial_x \\theta(x,\\,t) &= \\sum_{B=1}^n d_B\\, \\partial_x N_B(x) \\:+\\: \\theta_1 \\partial_x N_{n+1} \\quad, \\\\ \n",
    "\\partial_x \\tilde{\\theta}(x,\\,t) &= \\sum_{A=1}^n c_A\\,\\partial_x N_A \\quad,\n",
    "\\end{align*}\n",
    "\n",
    "where a dot above a variable indicates a derivative with respect to time. Note here that only the weights $c_A$ and $d_B$ are time dependent, while only the shape functions $N_i$ are spatially-varying. Finally,  $\\theta_1$ has no time dependence due to the boundary condition 7.81, \n",
    "\\begin{equation*}\n",
    "\\theta(1,\\,t) = \\theta_1 \\quad. \n",
    "\\end{equation*}\n",
    "Substituting in these summations to the heat equation produces \n",
    "\n",
    "\\begin{align*}\n",
    "    \\int_0^1 \\left(\\sum_{A=1}^n c_A\\,N_A \\right) \\, \\left( \\sum_{B=1}^n \\dot{d}_B\\,N_B \\right) \\: \\mathrm{d}x = - &\\int_0^1 \\alpha\\, \\left( \\sum_{A=1}^n c_A\\,\\partial_x N_A  \\right)  \\,\\left(\\sum_{B=1}^n d_B\\, \\partial_x N_B \\:+\\: \\theta_1 \\partial_x N_{n+1} \\right) \\: \\mathrm{d}x \\: \\\\ \n",
    "    + \\: &\\int_0^1 \\sum_{A=1}^n c_A\\,N_A \\, h\\, \\mathrm{d}x \\\\ \\: + &\\alpha\\, \\left[ \\tilde{\\theta} \\, \\partial_x \\theta \\,\\right]_0^1 \\quad. \n",
    "\\end{align*}\n",
    "\n",
    "Let us consider the different terms separately: \n",
    "\n",
    "#### Left-hand side\n",
    "The left-hand side can be re-ordered by removing the weights, which aren't spatially dependent, from the integral:  \n",
    "\n",
    "\\begin{align*}\n",
    "&\\int_0^1 \\left(\\sum_{A=1}^n c_A\\,N_A \\right) \\, \\left( \\sum_{B=1}^n \\dot{d}_B\\,N_B(x) \\right) \\: \\mathrm{d}x \\\\ \n",
    "&= \\sum_{A=1}^n \\sum_{B=1}^n  c_A\\,\\dot{d}_B\\int_0^1 N_A(x) \\,N_B(x) \\: \\mathrm{d}x \\\\\n",
    "&= \\sum_{A=1}^n \\sum_{B=1}^n c_A \\, M_{AB} \\, \\dot{d}_B  \\\\ \n",
    "\\end{align*}\n",
    "\n",
    "#### Right-hand side  - Term 1:\n",
    "We can similarly rearrange \n",
    "\n",
    "\\begin{align*}\n",
    "- &\\int_0^1 \\alpha\\, \\left( \\sum_{A=1}^n c_A\\,\\partial_x N_A  \\right)  \\,\\left(\\sum_{B=1}^n d_B\\, \\partial_x N_B \\:+\\: \\theta_1 \\partial_x N_{n+1} \\right) \\: \\mathrm{d}x \\\\ \n",
    "= - &\\int_0^1 \\alpha\\, \\left( \\sum_{A=1}^n c_A\\,\\partial_x N_A  \\right)  \\,\\left(\\sum_{B=1}^n d_B\\, \\partial_x N_B \\right) \\:+\\: \\alpha\\, \\left( \\sum_{A=1}^n c_A\\,\\partial_x N_A  \\right)  \\theta_1 \\partial_x N_{n+1}  \\: \\mathrm{d}x \\\\\n",
    "= - & \\sum_{A=1}^n \\sum_{B=1}^n c_A d_B \\int_0^1 \\alpha\\, \\left(  \\,\\partial_x N_A  \\right)  \\,\\left(\\, \\partial_x N_B \\right) \\: \\mathrm{d}x \\:-\\: \\sum_{A=1}^n c_A \\int_0^1 \\alpha\\, \\left( \\,\\partial_x N_A  \\right)  \\theta_1 \\left( \\partial_x N_{n+1} \\right) \\: \\mathrm{d}x \n",
    "\\end{align*}\n",
    "\n",
    "\n",
    "With Eqn. 7.86 this can then be written as \n",
    "\n",
    "\\begin{align*}\n",
    "= - & \\sum_{A=1}^n \\sum_{B=1}^n c_A K_{AB}\\, d_B  \\:-\\: \\sum_{A=1}^n c_A \\,\\theta_1 \\int_0^1 \\alpha\\, \\left( \\,\\partial_x N_A  \\right)   \\left( \\partial_x N_{n+1} \\right) \\: \\mathrm{d}x \n",
    "\\end{align*}\n",
    "\n",
    "\n",
    "#### Right-hand side  - Term 2:\n",
    "\n",
    "\\begin{align*}\n",
    "  &\\int_0^1 \\sum_{A=1}^n c_A\\,N_A \\, h\\, \\mathrm{d}x   \\\\ \n",
    "= & \\sum_{A=1}^n c_A \\int_0^1 \\,N_A \\, h\\, \\mathrm{d}x \\\\ \n",
    "\\end{align*}\n",
    "\n",
    "\n",
    "#### Right-hand side  - Term 3:\n",
    "Upon imposing the constraint of 7.21 that\n",
    "\\begin{equation*}\n",
    "\\tilde{\\theta}(1) = 0\\quad, \n",
    "\\end{equation*}\n",
    "this term reduces to \n",
    "\n",
    "\\begin{align*}\n",
    "\\alpha\\, \\left[ \\tilde{\\theta} \\, \\partial_x \\theta \\,\\right]_0^1 &= \\alpha(1)\\, \\tilde{\\theta}(1) \\, \\partial_x \\theta(1) - \\alpha(0)\\, \\tilde{\\theta}(0) \\, \\partial_x \\theta(0) \\\\ \n",
    "&=  - \\alpha(0) \\, \\tilde{\\theta}(0) \\, \\partial_x \\theta(0)\n",
    "\\end{align*}\n",
    "\n",
    "and using the boundary condition in Eqn 7.82 that \n",
    "\\begin{equation*}\n",
    "\\partial_x\\theta(0,\\,t) = - H_0 \\quad, \n",
    "\\end{equation*}\n",
    "\n",
    "this becomes \n",
    "\n",
    "\\begin{align*}\n",
    "&=   \\alpha(0) \\, H_0 \\, \\tilde{\\theta}(1) \\\\\n",
    "&=   \\sum_{A=1}^n c_A \\, N_A(1)\\, \\alpha(0) \\, H_0 \n",
    "\\end{align*}\n",
    "\n",
    "\n",
    "### Re-assembling the equation\n",
    "\n",
    "We can now write our global heat equation as \n",
    "\n",
    "\\begin{align*}\n",
    "\\sum_{A=1}^n \\sum_{B=1}^n c_A \\, M_{AB} \\, \\dot{d}_B = - & \\sum_{A=1}^n \\sum_{B=1}^n c_A K_{AB}\\, d_B  \\:-\\: \\sum_{A=1}^n c_A \\,\\theta_1 \\int_0^1 \\alpha\\, \\left( \\,\\partial_x N_A  \\right)   \\left( \\partial_x N_{n+1} \\right) \\: \\mathrm{d}x  \\\\ \n",
    "+ &  \\sum_{A=1}^n c_A \\int_0^1 \\,N_A \\, h\\, \\mathrm{d}x + \\sum_{A=1}^n c_A \\, N_A(0)\\, \\alpha(0) \\, H_0  \\quad. \n",
    "\\end{align*}\n",
    "\n",
    "By moving the term containing the diffusivity matrix to the LHS, we may write this as \n",
    "\n",
    "\n",
    "\\begin{align*}\n",
    "\\sum_{A=1}^n c_A \\left\\{ \\sum_{B=1}^n  \\, M_{AB} \\, \\dot{d}_B  +  \\sum_{B=1}^n  K_{AB}\\, d_B \\right\\} = \n",
    " \\sum_{A=1}^n c_A \\Big\\{&- \\,\\theta_1 \\int_0^1 \\alpha\\, \\left( \\,\\partial_x N_A  \\right)   \\left( \\partial_x N_{n+1} \\right) \\: \\mathrm{d}x  \\\\ \n",
    "&+   \\int_0^1 \\,N_A \\, h\\, \\mathrm{d}x + \\, N_A(0)\\, \\alpha(0) \\, H_0 \\Big\\} \\quad. \n",
    "\\end{align*}\n",
    "\n",
    "which can be simplified to \n",
    "\n",
    "\\begin{align*}\n",
    "\\sum_{A=1}^n c_A \\left\\{ \\sum_{B=1}^n  \\, M_{AB} \\, \\dot{d}_B  +  \\sum_{B=1}^n  K_{AB}\\, d_B \\right\\} = \n",
    " \\sum_{A=1}^n c_A F_A \\quad. \n",
    "\\end{align*}\n",
    "\n",
    "in which \n",
    "\\begin{equation*}\n",
    "F_A = - \\,\\theta_1 \\int_0^1 \\alpha\\, \\left( \\,\\partial_x N_A  \\right)   \\left( \\partial_x N_{n+1} \\right) \\: \\mathrm{d}x +   \\int_0^1 \\,N_A \\, h\\, \\mathrm{d}x + \\, N_A(0)\\, \\alpha(0) \\, H_0 \n",
    "\\end{equation*}\n",
    "\n",
    "**Note here the minor differences between the definition above and Eqn 7.87** \n",
    "\n",
    "\n",
    "### Probing the test function\n",
    "\n",
    "For the weak form to hold, the equations must hold for any test function $\\tilde{\\theta}$. Hence, we can probe the system of equations for different weak functions. This means that for any $C_A$\n",
    "\n",
    "\\begin{align*}\n",
    "\\sum_{A=1}^n c_A \\left\\{ \\sum_{B=1}^n  \\, M_{AB} \\, \\dot{d}_B  +  \\sum_{B=1}^n  K_{AB}\\, d_B \\right\\} = \n",
    " \\sum_{A=1}^n c_A F_A \\quad. \n",
    "\\end{align*}\n",
    "must hold. To probe this, let us consider each case $i = 1, n$ for which \n",
    "\n",
    "\\begin{equation*}\n",
    "C_A = \\begin{cases}\n",
    "1 & A=i \\\\\n",
    "0 & A\\ne i\n",
    "\\end{cases} \\quad.\n",
    "\\end{equation*}\n",
    "For this to hold, it requires that\n",
    "\n",
    "\\begin{align*}\n",
    " \\sum_{B=1}^n  \\, M_{AB} \\, \\dot{d}_B  +  \\sum_{B=1}^n  K_{AB}\\, d_B = \n",
    "  F_A \\quad\n",
    "\\end{align*}\n",
    "\n",
    "for every $A$. "
   ]
  }
 ],
 "metadata": {
  "kernelspec": {
   "display_name": "Python 3 (ipykernel)",
   "language": "python",
   "name": "python3"
  },
  "language_info": {
   "codemirror_mode": {
    "name": "ipython",
    "version": 3
   },
   "file_extension": ".py",
   "mimetype": "text/x-python",
   "name": "python",
   "nbconvert_exporter": "python",
   "pygments_lexer": "ipython3",
   "version": "3.8.10"
  }
 },
 "nbformat": 4,
 "nbformat_minor": 5
}
